linking/linking_proof2.v
@@ -321,7 +321,7 @@ Section vis_inv.
 Import Core.
 
 Record vis_inv (c : t cores_S) mu : Type :=
-  { vis_sup : {subset (RC.reach_basis my_ge c.(Core.c)) <= vis mu} }.
+  { vis_sup : {subset (RC.roots my_ge c.(Core.c)) <= vis mu} }.
 
 End vis_inv.
 
@@ -1411,7 +1411,7 @@ Lemma vis_inv_step (c c' : Core.t cores_S) :
 Proof.
 move=> E A B C rc; move: E.
 case=> E; apply: Build_vis_inv=> b F.
-move: F; rewrite/RC.reach_basis/in_mem/=; move/orP=> [|F].
+move: F; rewrite/RC.roots/in_mem/=; move/orP=> [|F].
 rewrite -A -B=> F. 
 by apply: (intern_incr_vis _ _ incr); apply: E; apply/orP; left.
 case G: (RC.locs (Core.c c) b). 
@@ -1425,7 +1425,7 @@ by move/sub1=> ->.
 by move=> ->; rewrite orb_comm.
 apply: rc; apply: (REACH_mono _ _ _ _ _ H)=> //.
 move=> b0 H2; move: (E b0); rewrite /in_mem /=; apply.
-apply: (RC.reach_basis_domains_eq _ H2).
+apply: (RC.roots_domains_eq _ H2).
 by apply: genvs_domain_eq_sym; apply: (my_ge_S (Core.i c)).
 Qed.
 
@@ -1647,7 +1647,7 @@ have atext1':
 move=> hd_match _.
 case: (core_at_external (sims (Core.i (c inv))) 
       _ _ _ _ _ _ hd_match atext1').
-move=> inj []defs1 []args2 []valinj []atext2 extends; exists args2.
+move=> inj []args2 []valinj []atext2 extends; exists args2.
 set T := C \o cores_T.
 rewrite /LinkerSem.at_external0.
 set P := fun ix (x : T ix) => 
@@ -1724,7 +1724,7 @@ have atext2'':
 
 case: (core_at_external (sims (Core.i (c inv))) 
       _ _ _ _ _ _ (head_match hdinv) atext1').
-move=> inj []defs1 []args2' []vinj []atext2''' extends.
+move=> inj []args2' []vinj []atext2''' extends.
 
 have eq: args2 = args2' by move: atext2'''; rewrite atext2''; case.
 subst args2'.
@@ -1745,6 +1745,11 @@ have j_domS_domT:
 
 have DomTgt_rc: REACH_closed m2 (DomTgt mu_top).
 { by move: (head_match hdinv)=> mtch; apply match_target in mtch. }
+
+have defs1: vals_def args1.
+{ clear - atext1'; move: atext1'; rewrite /= /RC.at_external.
+  case e: (at_external _ _)=> [[[ef0 dep_sig0] args0]|//].
+  by case f: (vals_def args0)=> //; case=> _ _ <-. }
 
 have frgnT_sub_domT: {subset frgnT <= domT}.
 { move=> b H; apply: DomTgt_rc. 
@@ -1951,7 +1956,7 @@ have mu_new_rel_inv_all:
 have mu_new_vis_inv: vis_inv c1 mu_new'.
 { apply: Build_vis_inv=> // b; rewrite /in_mem /= => Y.
   rewrite /vis /mu_new /frgnS /exportedSrc /=.
-  move: Y; rewrite /RC.reach_basis; case/orP.
+  move: Y; rewrite /RC.roots; case/orP.
   case/orP. case/orP. move=> H1.
   have H1': isGlobalBlock (ge (cores_S' (Core.i c1))) b.
   { by rewrite -isGlob_iffS. }
@@ -2712,31 +2717,31 @@ have subF: {subset frgnBlocksSrc mu0 <= frgnSrc'}.
   by rewrite /in_mem /= => ->; apply/orP; right.
   by apply: REACH_nil; apply/orP; right; apply/orP; left.
   by apply: nu'_wd. }
-{(*{subset RC.reach_basis ...}*)
+{(*{subset RC.roots ...}*)
   move: aft1'=> /= aft1'.
   move: (RC.after_external_rc_basis (ge (cores_S (Core.i hd1))) aft1').
   move=> eq_hd1' b; rewrite /in_mem /= => H.
   have eq_hd1'': 
-    RC.reach_basis (ge (cores_S (Core.i hd1'))) (Core.c hd1')
+    RC.roots (ge (cores_S (Core.i hd1'))) (Core.c hd1')
     = (fun b => 
          getBlocks [:: rv1] b
-      || RC.reach_basis (ge (cores_S (Core.i hd1))) (Core.c hd1) b).
+      || RC.roots (ge (cores_S (Core.i hd1))) (Core.c hd1) b).
   { move: eq_hd1'. 
     set T := C \o cores_S.
     set P := fun ix (x : T ix) => 
-               RC.reach_basis (ge (cores_S ix)) x 
+               RC.roots (ge (cores_S ix)) x 
            = (fun b0 => 
               getBlocks [:: rv1] b0
-              || RC.reach_basis (ge (cores_S (Core.i hd1))) (Core.c hd1) b0).
+              || RC.roots (ge (cores_S (Core.i hd1))) (Core.c hd1) b0).
     change (P (Core.i hd1) (cast T (sym_eq e1) (Core.c hd1'))
          -> P (Core.i hd1') (Core.c hd1')).
     by apply: cast_indnatdep'. }
   have eq_hd1''': 
-    RC.reach_basis my_ge (Core.c hd1') 
+    RC.roots my_ge (Core.c hd1') 
     = (fun b =>
          getBlocks [:: rv1] b
-         || RC.reach_basis (ge (cores_S (Core.i hd1))) (Core.c hd1) b).
-  { rewrite -eq_hd1'' /RC.reach_basis; extensionality b0.
+         || RC.roots (ge (cores_S (Core.i hd1))) (Core.c hd1) b).
+  { rewrite -eq_hd1'' /RC.roots; extensionality b0.
     have glob_eq: isGlobalBlock my_ge b0
                 = isGlobalBlock (ge (cores_S (Core.i hd1'))) b0. 
     { suff: isGlobalBlock my_ge b0 
@@ -2766,7 +2771,7 @@ have subF: {subset frgnBlocksSrc mu0 <= frgnSrc'}.
   { move=> RB; case: (frame_vis fr0)=> vis_sub. 
     have vis0_b: vis mu0 b.
     { apply: vis_sub.
-      rewrite /in_mem /=; move: RB; rewrite /RC.reach_basis.
+      rewrite /in_mem /=; move: RB; rewrite /RC.roots.
       have glob_eq: isGlobalBlock my_ge b
                   = isGlobalBlock (ge (cores_S (Core.i hd1))) b. 
       { suff: isGlobalBlock my_ge b 
@@ -2782,7 +2787,7 @@ have subF: {subset frgnBlocksSrc mu0 <= frgnSrc'}.
       by rewrite -glob_eq. }
     { case: (orP vis0_b); first by move=> ->.
       by move=> L; apply/orP; right; apply: subF. } } 
-}(*END {subset RC.reach_basis ...}*)
+}(*END {subset RC.roots ...}*)
 }(*END vis_inv*)
 }(*END head_inv*)
 
@@ -2981,7 +2986,7 @@ eapply Build_Wholeprog_simulation_inject
   exists erefl,mu_top,[::]=> /=; split=> //.
 
   exists erefl; apply: Build_head_inv=> //.
-  apply: Build_vis_inv; rewrite /= /RC.reach_basis /vis /mu_top0 /= /fS.
+  apply: Build_vis_inv; rewrite /= /RC.roots /vis /mu_top0 /= /fS.
 
   have ->: RC.args c = vals1.
   { by apply: (RC.initial_core_args g). }
